experiments/002_ssa_cfg/SirLean/Spec.lean
@@ -1,27 +1,17 @@
 import SirLean.Proof
-import SirLean.SmallStep
 
 namespace Sir
 
--- theorem BasicBlock.eval?_isSome : (BasicBlock.eval? bb w).isSome = true :=
---   BasicBlock.eval?_isSome.proof
--- 
--- def BasicBlock.eval (bb : BasicBlock) (w : World) := (bb.eval? w).get (BasicBlock.eval?_isSome)
--- 
--- def BasicBlock.execStart (bb : BasicBlock) (w : World) : BlockExecState bb :=
---   let pos :=
---     if h : 0 < bb.ops.size
---     then .op ⟨0, h⟩
---     else .last
---   { env := BasicBlock.initialCtx w, pos := pos }
--- 
--- def BasicBlock.execEnd (bb : BasicBlock) (w : World) : BlockExecState bb :=
---   let (env, t) := bb.eval w
---   { env := env, pos := .terminated t }
--- 
--- theorem BasicBlock.eval_is_blockSteps (bb : BasicBlock) (w : World) :
---     BlockSteps (bb.execStart w) (bb.execEnd w) := by
---   simp [BasicBlock.execStart, BasicBlock.execEnd, BasicBlock.eval]
---   exact BasicBlock.eval_is_blockSteps_proof bb w
+theorem ControlFlowGraph.eval?_iff_steps
+    (cfg : ControlFlowGraph) (w : World) (t : Termination) (w' : World) :
+    (∃ fuel, cfg.eval? w fuel = .ok (t, w')) ↔
+      CFGSteps cfg (cfg.initialConf w) (.done t w') :=
+  ControlFlowGraph.eval?_iff_steps.proof cfg w t w'
+
+theorem ControlFlowGraph.progress
+    (cfg : ControlFlowGraph) (w : World) (c : Conf)
+    (hreach : CFGSteps cfg (cfg.initialConf w) c) :
+    (∃ t w', c = .done t w') ∨ (∃ c', StepCFG cfg c c') :=
+  ControlFlowGraph.progress.proof cfg w c hreach
 
 end Sir
